theories/Example.v
@@ -4,7 +4,7 @@
 
 From Coq Require Import Bool String List BinPos Compare_dec Omega.
 From Equations Require Import Equations DepElimDec.
-From Template Require Import Ast LiftSubst Typing Checker Template.
+From Template Require Import Ast LiftSubst Typing Checker.
 From Translation Require Import util SAst SLiftSubst SCommon ITyping
                                 ITypingLemmata ITypingAdmissible XTyping
                                 Translation Pruning FinalTranslation
